\begin{equation}
    t = t + 1 
    \label{eq:1}
\end{equation}
\begin{equation}
    m_t = \beta_1 \cdot m_{t-1} + (1 - \beta_1) \cdot \nabla_{\theta} J(\theta) 
    \label{eq:2}
\end{equation}
\begin{equation}
    v_t = \beta_2 \cdot v_{t-1} + (1 - \beta_2) \cdot (\nabla_{\theta} J(\theta))^2 \label{eq:3}
\end{equation}
\begin{equation}
    \hat{m}_t = \frac{m_t}{1 - \beta_1^t}
    \label{eq:4}
\end{equation}
\begin{equation}
    \hat{v}_t = \frac{v_t}{1 - \beta_2^t}
    \label{eq:5}
\end{equation}
\begin{equation}
    \theta = \theta - \alpha \cdot \frac{\hat{m}_t}{\sqrt{\hat{v}_t} + \epsilon}
    \label{eq:6}
\end{equation}